src/PlutusIR/Semantics/Static/NoDup'_prototype.v
@@ -1,0 +1,597 @@
+From Coq Require Import Lists.List.
+From Coq Require Import Strings.String.
+
+From PlutusCert Require Import Util.List util.
+
+Import ListNotations.
+Local Open Scope list_scope.
+Local Open Scope string_scope.
+
+Lemma empty_concat : forall (A : Type), (([] : list A) = [] ++ [])%list.
+Proof.
+  intros A. 
+  simpl. reflexivity.
+Qed.
+
+
+
+(** kinds *)
+Inductive kind :=
+  | Kind_Base : kind
+  | Kind_Arrow : kind -> kind -> kind.
+
+(** Types *)
+Inductive ty :=
+  | Ty_Var : string -> ty
+  | Ty_Lam : string -> kind -> ty -> ty
+  | Ty_App : ty -> ty -> ty
+.
+
+(** Normal types *)
+Inductive normal_Ty : ty -> Prop :=
+  | NO_TyLam : forall bX K T,
+      normal_Ty T ->
+      normal_Ty (Ty_Lam bX K T)
+  | NO_neutral : forall T,
+      neutral_Ty T ->
+      normal_Ty T
+
+with neutral_Ty : ty -> Prop :=
+  | NE_TyVar : forall X,
+      neutral_Ty (Ty_Var X)
+  | NE_TyApp : forall T1 T2,
+      neutral_Ty T1 ->
+      normal_Ty T2 ->
+      neutral_Ty (Ty_App T1 T2).
+
+Fixpoint kind_eq (K1 K2 : kind) : bool :=
+    match K1, K2 with
+    | Kind_Base, Kind_Base => true
+    | Kind_Arrow K11 K12, Kind_Arrow K21 K22 =>
+        if kind_eq K11 K21 then
+            kind_eq K12 K22
+        else false
+    | _, _ => false
+    end.
+
+Fixpoint ty_eq (T1 T2 : ty) : bool :=
+    match T1, T2 with
+    | Ty_Var x1, Ty_Var x2 => if string_dec x1 x2 then true else false
+    | Ty_Lam x1 K1 T1', Ty_Lam x2 K2 T2' =>
+        if string_dec x1 x2 then
+            if (kind_eq K1 K2) then
+                ty_eq T1' T2'
+            else false
+        else false
+    | Ty_App T11 T12, Ty_App T21 T22 =>
+        if ty_eq T11 T21 then
+            ty_eq T12 T22
+        else false
+    | _, _ => false
+    end.
+
+Fixpoint btv (T : ty) : (list string) :=
+    match T with
+    | Ty_Var x => []
+    | Ty_Lam x K T0 => x :: (btv T0)
+    | Ty_App T1 T2 => btv T1 ++ btv T2
+    end.
+
+
+Fixpoint drop_btv (Δ : list (string * kind)) (btvs : list string) : list (string * kind) :=
+    match Δ with
+    | ((X, K)::Δ') => 
+                    if (in_dec string_dec X btvs) then
+                        (drop_btv Δ' btvs)
+                      else
+                        ((X, K)::(drop_btv Δ' btvs))
+    | nil => nil
+    end.
+
+
+Fixpoint lookup {X:Type} (k : string) (l : list (string * X)) : option X :=
+  match l with
+  | nil => None
+  | (j,x) :: l' => if j =? k then Datatypes.Some x else lookup k l'
+  end.
+
+  (* Maybe instead: if T is well_kinded and an application, then there is no capture*)
+(* Theorem well_kinded__no_capture2 Δ T1 T2 K :
+    (Δ |-* (Ty_App T1 T2) : K) -> (In X (ftv T2)) -> (~ In X (btv T1)). *)
+
+Fixpoint substituteT (X : string) (U T : ty) : ty :=
+  match T with
+  | Ty_Var Y =>
+    if X =? Y then U else Ty_Var Y
+  | Ty_Lam Y K1 T' =>
+    if X =? Y then Ty_Lam Y K1 T' else Ty_Lam Y K1 (substituteT X U T')
+  | Ty_App T1 T2 =>
+    Ty_App (substituteT X U T1) (substituteT X U T2)
+  end.
+
+(* It may already be present, but only with the same body *)
+Definition P_ND (X : string) (T : ty) (Δ : list (string * ty)) := 
+  forall T', lookup X Δ = Some T' -> T = T'.
+
+(* Not strong enough. Even when shadowed things have different T, it is a problem*)
+Definition P_ND2 (Δ1 Δ2 : list (string * ty)) :=
+    forall X T T', lookup X Δ1 = Some T -> lookup X Δ2 = Some T' -> T <> T' -> False.
+
+Definition P_ND2' (Δ1 Δ2 : list (string * ty)) :=
+    forall X T T', In (X, T) Δ1 -> In (X, T') Δ2 -> T <> T' -> False.
+
+(* If a binder occurs multiple times, and we started with a GU term,
+    we must have had a beta reduction. This we only do with normal types.
+*)
+Definition P_Dup_Normal (Δ1 Δ2 : list (string * ty)) :=
+    forall X T T', In (X, T) Δ1 -> In (X, T') Δ2 -> T = T' -> normal_Ty T.
+
+Definition P_BF (Δ : list (string * ty)) (Γ : list string) :=
+    forall X, In X Γ -> ~ In X (map fst Δ).
+
+(*
+    Δ keeps track of lambda bodies, to make sure we never have dissimilar bodies for the same binder
+    Γ keeps track of ftvs: no ftv may be bound somewhere else
+*)
+Reserved Notation "Δ : Γ '⊢' T" (at level 40, Γ at level 0, T at level 0, no associativity).
+Inductive WK_Dup' : list (string * ty) -> list string -> ty -> Prop :=
+  | ND_Var : forall Δ Γ X,
+      In X Γ ->
+      Δ : Γ ⊢ (Ty_Var X) 
+  | ND_Lam : forall Δ Γ X K1 T ,
+      Δ : (X::Γ) ⊢ T ->
+      
+      (* P_ND X T Δ ->  *)
+      (* Do we need this? *)
+      ((X, T)::Δ) : Γ ⊢ (Ty_Lam X K1 T)
+  | ND_App : forall Δ1 Δ2 Γ T1 T2 ,
+      Δ1 : Γ ⊢ T1 ->
+      Δ2 : Γ ⊢ T2 ->
+      P_ND2' Δ1 Δ2 ->
+      (* P_Dup_Normal Δ1 Δ2 -> *)
+      P_BF (Δ1 ++ Δ2) Γ ->
+      (Δ1 ++ Δ2) : Γ ⊢ (Ty_App T1 T2)
+where "Δ : Γ '⊢' T" := (WK_Dup' Δ Γ T).
+
+
+Create HintDb noDup_db.
+Hint Constructors WK_Dup' : noDup_db.
+
+Definition KB := Kind_Base.
+
+(* 
+(λX. λY. X Y)   (ΛY. Y)
+*)
+Definition t1_bad := Ty_App
+        ( Ty_Lam "X" KB (Ty_Lam "Y" KB (Ty_App (Ty_Var "X") (Ty_Var "Y"))))
+        (Ty_Lam "Y" KB (Ty_Var "Y")).
+
+Lemma t1_bad__not_wk :
+    forall Δ Γ,
+        (Δ : Γ ⊢ t1_bad) -> False.
+Proof.
+    intros.
+    unfold t1_bad in H.
+    inversion H; subst; clear H.
+    inversion H3; subst; clear H3.
+    inversion H2; subst; clear H2.
+    inversion H3; subst; clear H3.
+    contradiction H6 with (X := "Y") (T := Ty_App (Ty_Var "X") (Ty_Var "Y"))
+                (T' := (Ty_Var "Y")); auto with *.
+Qed.
+
+(* 
+(λW.  (λZ. W Z) (λY. Y))   (λX. λY. X Y)
+This term multisteps to t1_bad *)
+Definition t2_bad := Ty_App
+        (Ty_Lam "W" KB (Ty_App 
+                (Ty_Lam "Z" KB (Ty_App (Ty_Var "W") (Ty_Var "Z")))
+                (Ty_Lam "Y" KB (Ty_Var "Y"))))
+        (Ty_Lam "X" KB (Ty_Lam "Y" KB (Ty_App (Ty_Var "X") (Ty_Var "Y")))).
+
+Lemma t2_bad__not_wk :
+    forall Δ Γ,
+        (Δ : Γ ⊢ t2_bad) -> False.
+Proof.
+    intros.
+    unfold t2_bad in H.
+    inversion H; subst; clear H.
+    inversion H2; subst; clear H2.
+    inversion H4; subst; clear H4.
+    inversion H1; subst; clear H1.
+    inversion H2; subst; clear H2.
+    inversion H3; subst; clear H3.
+    inversion H2; subst; clear H2.
+
+    contradiction H6 with (X := "Y") (T := (Ty_Var "Y")) (T' := (Ty_App (Ty_Var "X") (Ty_Var "Y"))).
+    all: auto with *.
+Qed.
+
+Definition t2_good := Ty_App
+        (Ty_Lam "X" KB (Ty_App (Ty_Lam "Y" KB (Ty_App (Ty_Var "Y") (Ty_Var "X"))) (Ty_Lam "Z" KB (Ty_Var "X"))))
+        (Ty_Lam "V" KB (Ty_Var "V")).
+
+Lemma t2_good__wk :
+    exists Δ,
+        (Δ : nil ⊢ t2_good).
+Proof with eauto with noDup_db.
+    exists (
+            (
+             ("X", (Ty_App (Ty_Lam "Y" KB (Ty_App (Ty_Var "Y") (Ty_Var "X"))) (Ty_Lam "Z" KB (Ty_Var "X"))))
+            ::([("Y", (Ty_App (Ty_Var "Y") (Ty_Var "X")))]
+            ++ ("Z", (Ty_Var "X"))::nil))
+            ++
+            [("V", (Ty_Var "V"))])%list.
+    unfold t2_good.
+    apply ND_App.
+    - apply ND_Lam.
+      apply ND_App.
+      apply ND_Lam.
+      rewrite empty_concat.
+      constructor.
+      constructor. apply in_eq. constructor. apply in_cons. apply in_eq.
+      
+      unfold P_ND2'. intros. inversion H.
+      unfold P_BF. intros. intros Hcontra. simpl in Hcontra. assumption.
+      apply ND_Lam.
+      constructor. apply in_cons. apply in_eq.
+      unfold P_ND2'. intros. inversion H0. inversion H2. subst.
+      inversion H. inversion H3. inversion H3.
+      inversion H2.
+      unfold P_BF. intros. inversion H. subst. intros Hcontra.
+      simpl in Hcontra.
+      inversion Hcontra.
+      congruence.
+      inversion H0.
+      congruence.
+      exact H1.
+      inversion H0.
+    - apply ND_Lam.
+      constructor. apply in_eq.
+    - unfold P_ND2'. intros.
+      inversion H0.
+      2: inversion H2.
+      inversion H2; subst.
+      
+      inversion H. inversion H3. inversion H3.
+      inversion H4. inversion H4. inversion H5. inversion H5.
+    - unfold P_BF.
+      intros.
+      inversion H.
+Qed.
+
+(* PROBLEM: open terms
+    (λ x λ y. x y ) (v y) would cause capture.
+
+    Maybe fixed by adding Γ
+*)
+
+Definition t3_bad := Ty_App
+        (Ty_Lam "X" KB (Ty_Lam "Y" KB (Ty_App (Ty_Var "X") (Ty_Var "Y"))))
+        (Ty_App (Ty_Var "v") (Ty_Var "Y")).
+
+Lemma t3_bad__not_wk :
+    forall Δ Γ,
+        (Δ : Γ ⊢ t3_bad) -> False.
+Proof.
+    intros.
+    unfold t3_bad in H.
+    inversion H; subst; clear H.
+    inversion H2; subst; clear H2.
+    inversion H4; subst; clear H4.
+
+    (*But Y must be in Γ*)
+    inversion H3; subst; clear H3.
+    inversion H4; subst; clear H4.
+
+    contradiction H7 with (X := "Y").
+    all: auto with *.
+    simpl.
+    right.
+    left.
+    reflexivity.
+Qed.
+
+(* This term steps to t3_bad *)
+Definition t4_bad := Ty_App
+    (Ty_Lam "W" KB ( Ty_App
+        (Ty_Lam "X" KB (Ty_Lam "Y" KB (Ty_App (Ty_Var "X") (Ty_Var "Y"))))
+        (Ty_Var "W")
+    ))
+    (Ty_App (Ty_Var "v") (Ty_Var "Y")).
+
+Lemma t4_bad__not_wk :
+    forall Δ Γ,
+        (Δ : Γ ⊢ t4_bad) -> False.
+Proof.
+    intros.
+    unfold t4_bad in H.
+    inversion H; subst; clear H.
+    inversion H2; subst; clear H2.
+    inversion H4; subst; clear H4.
+    inversion H1; subst; clear H1.
+    inversion H5; subst; clear H5.
+
+    (*But Y must be in Γ*)
+    inversion H3; subst; clear H3.
+    inversion H5; subst; clear H5.
+
+    contradiction H7 with (X := "Y").
+    simpl.
+    right. right. left.
+    reflexivity.
+Qed.
+
+
+(** Kinding of types *)
+Reserved Notation "Δ '|-*' T ':' K" (at level 40, T at level 0, K at level 0).
+Inductive has_kind : list (string * kind) -> ty -> kind -> Prop :=
+  | K_Var : forall Δ X K,
+      lookup X Δ = Some K ->
+      Δ |-* (Ty_Var X) : K
+  | K_Lam : forall Δ X K1 T K2,
+      ((X, K1) :: Δ) |-* T : K2 ->
+      Δ |-* (Ty_Lam X K1 T) : (Kind_Arrow K1 K2)
+  | K_App : forall Δ T1 T2 K1 K2,
+      Δ |-* T1 : (Kind_Arrow K1 K2) ->
+      (drop_btv Δ (btv T1)) |-* T2 : K1 -> (* This rule makes that a well-kinded type can never have capture when evaluated one step*)
+      Δ |-* (Ty_App T1 T2) : K2
+where "Δ '|-*' T ':' K" := (has_kind Δ T K).
+
+Theorem well_kinded__no_capture :
+    (* Maybe:
+        Then if T is well_kinded with above has_kind,
+        then it is also well_kinded with canonical has_kind
+        And that then they normalise to same type?
+
+        Probably, but seems like a lot of work.
+    *) True
+.
+
+
+  (* Usual step relation that has no normality restrictions, 
+    but with naive subsitutions.
+*)
+Inductive step : ty -> ty -> Set :=
+    | step_beta (X : string) (K : kind) (S T : ty) :
+        normal_Ty S ->
+        normal_Ty T ->
+        step (Ty_App (Ty_Lam X K S) T) (substituteT X T S) 
+    | step_appL S1 S2 T :
+        step S1 S2 -> step (Ty_App S1 T) (Ty_App S2 T)
+    | step_appR S T1 T2 :
+        normal_Ty S ->
+        step T1 T2 -> step (Ty_App S T1) (Ty_App S T2)
+    | step_abs bX K T1 T2 :
+        step T1 T2 -> step (Ty_Lam bX K T1) (Ty_Lam bX K T2)
+    .
+
+(* HMM, I do not seem to use this for open U? *)
+Theorem substituteT_preserves_kinding : forall T Delta X K U L,
+  ((X, L) :: Delta) |-* T : K ->
+  (drop_btv Delta (btv T)) |-* U : L -> (* This lemma is used where X was in a lambda binder: hence, by the new typing rule, it may not occur free in U*)
+  Delta |-* (substituteT X U T) : K.
+Proof with eauto.
+  induction T.
+  all: intros Delta X K U L Hkind__T HHkind__U.
+  all: simpl.
+  all: inversion Hkind__T; subst...
+  - (* Ty_Var *)
+    destruct (X =? s)%string eqn:Heqb.
+    + (* X = Y *)
+      apply eqb_eq in Heqb as Heq.
+      subst.
+      assert (K = L).
+      {
+        simpl in H1.
+        rewrite Heqb in H1.
+        inversion H1; auto.
+      }
+      subst.
+      (* ADMIT: weakening *)
+      admit.
+    + (* X <> Y *)
+      apply eqb_neq in Heqb as Hneq.
+      rewrite lookup_neq in H1...
+      constructor.
+      assumption.
+  - (* Ty_Lam *)
+    rename s into bX.
+    destruct (X =? bX)%string eqn:Heqb.
+    + (* X = bX *)
+      apply eqb_eq in Heqb as Heq.
+      subst.
+      apply K_Lam...
+      (* ADMIT: Weakening shadow *)
+      admit.
+    + (* X <> bX *)
+      apply eqb_neq in Heqb as Hneq.
+      apply K_Lam.
+      eapply IHT...
+      * (* ADMIT: Weakening cons permute *)
+        admit.
+      * simpl.
+        destruct (in_dec string_dec bX (btv T)); eauto.
+        -- (* ADMIT: Weakening: now bX could be added to it, but it cannot shadow*)
+           admit.
+        -- (* U is well_kinded without bX, so we can add it without shadowing *)
+           admit.
+  - (* Ty_App *)
+    apply K_App with (K1 := K1).
+    + eapply IHT1...
+      admit.
+    + eapply IHT2...
+      * (* If U contains btvs free in T2, then it all fails *)
+        admit.
+      * admit.
+    
+Admitted.
+
+
+
+
+Fixpoint Δ_step (Δ : list (string * ty)) (T1 T2 : ty) : list (string * ty) :=
+    match Δ with
+    | nil => nil
+    | (X, T)::Δ' =>
+        if ty_eq T T1 then
+            (X, T2)::(Δ_step Δ' T1 T2)
+        else
+            Δ_step Δ' T1 T2
+    end.
+
+Lemma Δ_step_app_rewrite : forall Δ1 Δ2 T1 T2,
+    Δ_step (Δ1 ++ Δ2) T1 T2 = ((Δ_step Δ1 T1 T2) ++ (Δ_step Δ2 T1 T2))%list.
+Admitted.
+
+(* HMM, I do not seem to use this for open U? *)
+Theorem substituteT_preserves_NoDup : forall T Δ1 Δ2 Γ X U,
+  normal_Ty T ->
+  normal_Ty U ->
+  Δ1 : (X :: Γ) ⊢ T ->
+  Δ2 : Γ ⊢ U -> (* This lemma is used where X was in a lambda binder: hence, by the new typing rule, it may not occur free in U*)
+  Δ1 : Γ ⊢ (substituteT X U T).
+Proof with eauto.
+    intros T Δ1 Δ2 Γ X U HNo_T HNo_U HndT HndU.
+    generalize dependent Δ2.
+    generalize dependent Δ1.
+    generalize dependent Γ.
+    induction T.
+    - intros.
+      simpl.
+      destr_eqb_eq X s.
+      + admit.
+      + eexists.
+        constructor.
+        inversion HndT.
+        subst.
+        inversion H3; subst.
+        congruence.
+        auto.
+    - intros.
+      simpl.
+      destr_eqb_eq X s.
+      + (* X = s*)
+        inversion HndT; subst.
+        eexists.
+        constructor.
+        (* Some weakening argument*)
+        admit.
+      + (* X <> s *)
+        inversion HndT; subst.
+        assert ((s, T) = (s, substituteT X U T)).
+        {
+            (* This is a problem *)
+            admit.
+        }
+        assert (WK_Dup' Δ (X :: s :: Γ) T).
+        {
+            (* Some weakening argument*)
+            admit.
+        }
+        inversion HNo_T; subst.
+        specialize (IHT H4 _ _ H1).
+        assert (WK_Dup' Δ2 (s :: Γ) U).
+        {
+            (* Some weakening argument*)
+            admit.
+        }
+        specialize (IHT _ H2) as [Δ0 HndΔ0].
+        exists ((s, substituteT X U T)::Δ0).
+        apply ND_Lam.
+        assumption.
+
+        (* lam cannot be neutral *)
+        inversion H2.
+    - intros.
+      simpl.
+      inversion HndT; subst.
+      inversion HNo_T; subst.
+      inversion H; subst.
+      apply NO_neutral in H5.
+      specialize (IHT1 H5 _ _ H1 _ HndU) as [Δ1' IHT1].
+      specialize (IHT2 H8 _ _ H2 _ HndU) as [Δ2' IHT2].
+      exists (Δ1' ++ Δ2')%list.
+      constructor; eauto.
+      + admit.
+      + admit.
+      + admit.
+
+Admitted.
+
+(* This is the property that we want to prove: that the step relation preserves the typing property *)
+Theorem preservation' T1 T2 Δ Γ :
+    Δ : Γ ⊢ T1 -> step T1 T2 -> exists Δ', Δ' : Γ ⊢ T2.
+Proof.
+    intros Hnd Hstep.
+    generalize dependent Δ.
+    generalize dependent Γ.
+    induction Hstep; intros.
+    - inversion Hnd; subst.
+      inversion H1; subst.
+      eapply substituteT_preserves_NoDup; eauto.
+    - (* Analogous to below *)
+      admit.
+    - inversion Hnd; subst.
+      specialize (IHHstep Γ Δ2 H2) as [Δ2' Hnd2'].
+      exists (Δ1 ++ Δ2')%list.
+      constructor; auto.
+      + (* Something, say (X, T) in Δ2' stepped. so we could have lost this property if 
+            X is a key in Δ1. 
+            But by P_Dup_Normal, we know that then it could not have stepped (by normality).
+        *)
+        admit.
+      + (* Something in Δ2 could have stepped. But only if it didnt already occur in Δ1 by normality *)
+        admit.
+      + (* Δ2' is obtained from Δ2 by stepping. Hence bvs Δ2' are subset of bvs Δ2, so no problem*)
+        admit.
+    - inversion Hnd; subst.
+      specialize (IHHstep (bX :: Γ) Δ0 H2) as [Δ0' Hnd0'].
+      exists ((bX, T2)::Δ0')%list.
+      constructor; auto.
+Admitted.
+
+(* Even after stepping, the type is still typeable in the more restrictive TyApp rule
+  meaning that even after stepping, when stepping again, we will again not have capture
+  i.e. this is the property that GU implies that is preserved
+  under normalisation/betaReduction.
+*)
+Theorem preservation T1 T2 Δ K :
+    Δ |-* T1 : K -> step T1 T2 -> Δ |-* T2 : K.
+Proof.
+    intros Hwk Hstep.
+    generalize dependent Δ.
+    generalize dependent K.
+    induction Hstep; intros.
+    - inversion Hwk; subst.
+      inversion H2; subst.
+      assert ((drop_btv Δ (btv S)) |-* T : K1).
+      {
+        (* Weakening, we coulud potentially add X, but it cannot be free in T by H4*)
+        admit.
+      }
+      eapply substituteT_preserves_kinding; eauto.
+    - inversion Hwk; subst.
+      apply K_App with (K1 := K1).
+      + eapply IHHstep; eauto.
+      + (* stepping does not introduce new btvs, 
+        but it could remove them, hence
+            btv S2  subset of  btv S1
+
+            Hence 
+               inclusion (drop_btv Δ (btv s1)) (drop_btv Δ (btv s2))
+            reasoning: btv s1 is bigger than btv s2: we remove more, hence lookup in the first implies still lookup in the second, which has every element in the first, and possibly more
+
+            But what about shadowing??? I fear the existence of an X that becomes visible, but then that X was not necessary to begin with. So no issue.
+
+        *)
+        admit.
+    - inversion Hwk; subst.
+      apply K_App with (K1 := K1).
+      + assumption.
+      + eapply IHHstep; eauto.
+    - inversion Hwk; subst.
+      constructor.
+      eapply IHHstep; eauto.
+      
+Admitted.
