src/PlutusIR/Semantics/Static/NoDup'_prototype_normalise.v
@@ -1,0 +1,739 @@
+From Coq Require Import Lists.List.
+From Coq Require Import Strings.String.
+
+From PlutusCert Require Import Util.List util.
+
+Import ListNotations.
+Local Open Scope list_scope.
+Local Open Scope string_scope.
+
+Lemma empty_concat : forall (A : Type), (([] : list A) = [] ++ [])%list.
+Proof.
+  intros A. 
+  simpl. reflexivity.
+Qed.
+
+
+
+(** kinds *)
+Inductive kind :=
+  | Kind_Base : kind
+  | Kind_Arrow : kind -> kind -> kind.
+
+(** Types *)
+Inductive ty :=
+  | Ty_Var : string -> ty
+  | Ty_Lam : string -> kind -> ty -> ty
+  | Ty_App : ty -> ty -> ty
+.
+
+(** Normal types *)
+Inductive normal_Ty : ty -> Prop :=
+  | NO_TyLam : forall bX K T,
+      normal_Ty T ->
+      normal_Ty (Ty_Lam bX K T)
+  | NO_neutral : forall T,
+      neutral_Ty T ->
+      normal_Ty T
+
+with neutral_Ty : ty -> Prop :=
+  | NE_TyVar : forall X,
+      neutral_Ty (Ty_Var X)
+  | NE_TyApp : forall T1 T2,
+      neutral_Ty T1 ->
+      normal_Ty T2 ->
+      neutral_Ty (Ty_App T1 T2).
+
+(* Maybe instead: if T is well_kinded and an application, then there is no capture*)
+(* Theorem well_kinded__no_capture2 Δ T1 T2 K :
+    (Δ |-* (Ty_App T1 T2) : K) -> (In X (ftv T2)) -> (~ In X (btv T1)). *)
+Fixpoint substituteT (X : string) (U T : ty) : ty :=
+  match T with
+  | Ty_Var Y =>
+    if X =? Y then U else Ty_Var Y
+  | Ty_Lam Y K1 T' =>
+    if X =? Y then Ty_Lam Y K1 T' else Ty_Lam Y K1 (substituteT X U T')
+  | Ty_App T1 T2 =>
+    Ty_App (substituteT X U T1) (substituteT X U T2)
+  end.
+
+(** Type normalisation *)
+Inductive normalise : ty -> ty -> Prop :=
+  | N_BetaReduce : forall bX K T1 T2 T1n T2n T,
+      normalise T1 (Ty_Lam bX K T1n) ->    
+      normalise T2 T2n ->
+      normalise (substituteT bX T2n T1n) T ->
+      normalise (Ty_App T1 T2) T
+  | N_TyApp : forall T1 T2 T1n T2n,
+      normalise T1 T1n ->
+      neutral_Ty T1n ->
+      normalise T2 T2n ->
+      normalise (Ty_App T1 T2) (Ty_App T1n T2n)
+  | N_TyLam : forall bX K T0 T0n,
+      normalise T0 T0n ->
+      normalise (Ty_Lam bX K T0) (Ty_Lam bX K T0n)
+  | N_TyVar : forall X,
+      normalise (Ty_Var X) (Ty_Var X)
+  .
+
+
+Fixpoint kind_eq (K1 K2 : kind) : bool :=
+    match K1, K2 with
+    | Kind_Base, Kind_Base => true
+    | Kind_Arrow K11 K12, Kind_Arrow K21 K22 =>
+        if kind_eq K11 K21 then
+            kind_eq K12 K22
+        else false
+    | _, _ => false
+    end.
+
+Fixpoint ty_eq (T1 T2 : ty) : bool :=
+    match T1, T2 with
+    | Ty_Var x1, Ty_Var x2 => if string_dec x1 x2 then true else false
+    | Ty_Lam x1 K1 T1', Ty_Lam x2 K2 T2' =>
+        if string_dec x1 x2 then
+            if (kind_eq K1 K2) then
+                ty_eq T1' T2'
+            else false
+        else false
+    | Ty_App T11 T12, Ty_App T21 T22 =>
+        if ty_eq T11 T21 then
+            ty_eq T12 T22
+        else false
+    | _, _ => false
+    end.
+
+Fixpoint btv (T : ty) : (list string) :=
+    match T with
+    | Ty_Var x => []
+    | Ty_Lam x K T0 => x :: (btv T0)
+    | Ty_App T1 T2 => btv T1 ++ btv T2
+    end.
+
+Fixpoint ftv_ignore_lam (T : ty) : (list string) :=
+    match T with
+    | Ty_Var x => [x]
+    | Ty_Lam x K T0 => [] (* Where we call this, we know there are no lams. *)
+    | Ty_App T1 T2 => ftv_ignore_lam T1 ++ ftv_ignore_lam T2
+    end.
+
+Fixpoint drop_btv (Δ : list (string * kind)) (btvs : list string) : list (string * kind) :=
+    match Δ with
+    | ((X, K)::Δ') => 
+                    if (in_dec string_dec X btvs) then
+                        (drop_btv Δ' btvs)
+                      else
+                        ((X, K)::(drop_btv Δ' btvs))
+    | nil => nil
+    end.
+
+
+Fixpoint lookup {X:Type} (k : string) (l : list (string * X)) : option X :=
+  match l with
+  | nil => None
+  | (j,x) :: l' => if j =? k then Datatypes.Some x else lookup k l'
+  end.
+
+(* It may already be present, but only with the same body *)
+Definition P_ND (X : string) (T : ty) (Δ : list (string * ty)) := 
+  forall T', lookup X Δ = Some T' -> T = T'.
+
+(* Not strong enough. Even when shadowed things have different T, it is a problem*)
+Definition P_ND2 (Δ1 Δ2 : list (string * ty)) :=
+    forall X T T', lookup X Δ1 = Some T -> lookup X Δ2 = Some T' -> T <> T' -> False.
+
+Definition P_ND2' (Δ1 Δ2 : list (string * ty)) :=
+    forall X T T', In (X, T) Δ1 -> In (X, T') Δ2 -> T = T'.
+
+(* If a binder occurs multiple times, and we started with a GU term,
+    we must have had a beta reduction. This we only do with normal types.
+*)
+Definition P_Dup_Normal (Δ1 Δ2 : list (string * ty)) :=
+    forall X T T', In (X, T) Δ1 -> In (X, T') Δ2 -> T = T' -> normal_Ty T.
+
+Definition P_BF (Δ : list (string * ty)) (Γ : list string) :=
+    forall X, In X Γ -> ~ In X (map fst Δ).
+
+(*
+    Δ keeps track of lambda bodies, to make sure we never have dissimilar bodies for the same binder
+    Γ keeps track of ftvs: no ftv may be bound somewhere else
+*)
+Reserved Notation "Δ : Γ '⊢' T" (at level 40, Γ at level 0, T at level 0, no associativity).
+Inductive WK_Dup' : list (string * ty) -> list string -> ty -> Prop :=
+  | ND_Var : forall Γ X,
+      In X Γ ->
+      [] : Γ ⊢ (Ty_Var X)   (* I changed this to nil, so that we cannot have random stuff in there*)
+  | ND_Lam : forall Δ Γ X K1 T,
+      Δ : (X::Γ) ⊢ T ->
+      (* P_ND X T Δ ->  *)
+      (* Do we need this? *)
+      P_BF ((X, T)::Δ) Γ -> (* uhm *)
+      ((X, T)::Δ) : Γ ⊢ (Ty_Lam X K1 T)
+  | ND_App : forall Δ1 Δ2 Γ T1 T2 ,
+      Δ1 : Γ ⊢ T1 ->
+      Δ2 : Γ ⊢ T2 ->
+      P_ND2' Δ1 Δ2 ->
+      P_Dup_Normal Δ1 Δ2 ->
+      P_BF (Δ1 ++ Δ2) Γ ->
+      (Δ1 ++ Δ2) : Γ ⊢ (Ty_App T1 T2)
+where "Δ : Γ '⊢' T" := (WK_Dup' Δ Γ T).
+
+
+Create HintDb noDup_db.
+Hint Constructors WK_Dup' : noDup_db.
+
+Definition KB := Kind_Base.
+
+(* 
+(λX. λY. X Y)   (ΛY. Y)
+*)
+Definition t1_bad := Ty_App
+        ( Ty_Lam "X" KB (Ty_Lam "Y" KB (Ty_App (Ty_Var "X") (Ty_Var "Y"))))
+        (Ty_Lam "Y" KB (Ty_Var "Y")).
+
+Lemma t1_bad__not_wk :
+    forall Δ Γ,
+        (Δ : Γ ⊢ t1_bad) -> False.
+Proof.
+    intros.
+    unfold t1_bad in H.
+    inversion H; subst; clear H.
+    inversion H3; subst; clear H3.
+    inversion H2; subst; clear H2.
+    inversion H5; subst; clear H5.
+    unfold P_ND2' in H4.
+    specialize H4 with (X := "Y") (T := Ty_App (Ty_Var "X") (Ty_Var "Y"))
+                (T' := (Ty_Var "Y")).
+    discriminate H4; auto with *.
+Qed.
+
+(* 
+(λW.  (λZ. W Z) (λY. Y))   (λX. λY. X Y)
+This term multisteps to t1_bad *)
+Definition t2_bad := Ty_App
+        (Ty_Lam "W" KB (Ty_App 
+                (Ty_Lam "Z" KB (Ty_App (Ty_Var "W") (Ty_Var "Z")))
+                (Ty_Lam "Y" KB (Ty_Var "Y"))))
+        (Ty_Lam "X" KB (Ty_Lam "Y" KB (Ty_App (Ty_Var "X") (Ty_Var "Y")))).
+
+Lemma t2_bad__not_wk :
+    forall Δ Γ,
+        (Δ : Γ ⊢ t2_bad) -> False.
+Proof.
+    intros.
+    unfold t2_bad in H.
+    inversion H; subst; clear H.
+    inversion H2; subst; clear H2.
+    inversion H3; subst; clear H3.
+    inversion H5; subst; clear H5.
+    inversion H6; subst; clear H6.
+    inversion H2; subst; clear H2.
+    unfold P_ND2' in H4.
+
+    specialize H4 with (X := "Y") (T := (Ty_Var "Y")) (T' := (Ty_App (Ty_Var "X") (Ty_Var "Y"))).
+    discriminate H4; auto with *.
+Qed.
+
+Definition t2_good := Ty_App
+        (Ty_Lam "X" KB (Ty_App (Ty_Lam "Y" KB (Ty_App (Ty_Var "Y") (Ty_Var "X"))) (Ty_Lam "Z" KB (Ty_Var "X"))))
+        (Ty_Lam "V" KB (Ty_Var "V")).
+
+Lemma t2_good__wk :
+    exists Δ,
+        (Δ : nil ⊢ t2_good).
+Proof with eauto with noDup_db.
+    exists (
+            (
+             ("X", (Ty_App (Ty_Lam "Y" KB (Ty_App (Ty_Var "Y") (Ty_Var "X"))) (Ty_Lam "Z" KB (Ty_Var "X"))))
+            ::([("Y", (Ty_App (Ty_Var "Y") (Ty_Var "X")))]
+            ++ ("Z", (Ty_Var "X"))::nil))
+            ++
+            [("V", (Ty_Var "V"))])%list.
+    unfold t2_good.
+    apply ND_App.
+    - apply ND_Lam.
+      apply ND_App.
+      apply ND_Lam.
+      rewrite empty_concat.
+      constructor.
+      constructor. apply in_eq. constructor. apply in_cons. apply in_eq.
+      
+      unfold P_ND2'. intros. inversion H.
+      unfold P_Dup_Normal. intros. inversion H.
+      unfold P_BF. intros. intros Hcontra. simpl in Hcontra. assumption.
+      unfold P_BF. intros. inversion H. subst. simpl. intuition. congruence. inversion H0.
+      apply ND_Lam.
+      constructor. apply in_cons. apply in_eq.
+      unfold P_BF. intros. inversion H. subst. simpl. intuition. congruence. inversion H0.
+      unfold P_ND2'. intros. inversion H0. inversion H1. subst.
+      inversion H. inversion H2. subst. inversion H2. inversion H1.
+      unfold P_Dup_Normal. intros. subst. inversion H0. inversion H1. subst.
+      inversion H. inversion H2. inversion H2. inversion H1.
+      unfold P_BF. intros. inversion H. subst. intros Hcontra.
+      simpl in Hcontra.
+      inversion Hcontra.
+      congruence.
+      inversion H0.
+      congruence.
+      exact H1.
+      inversion H0.
+      unfold P_BF. intros. inversion H.
+    - apply ND_Lam.
+      constructor. apply in_eq.
+      unfold P_BF. intros. inversion H.
+    - unfold P_ND2'. intros.
+      inversion H0.
+      2: inversion H1.
+      inversion H1; subst.
+      
+      inversion H. inversion H2. inversion H2.
+      inversion H3. inversion H3. inversion H4. inversion H4.
+    - unfold P_Dup_Normal.
+      intros.
+      subst. inversion H0. inversion H1. subst. constructor. constructor. inversion H1.
+    - unfold P_BF.
+      intros.
+      inversion H.
+Qed.
+
+(* PROBLEM: open terms
+    (λ x λ y. x y ) (v y) would cause capture.
+
+    Maybe fixed by adding Γ
+*)
+
+Definition t3_bad := Ty_App
+        (Ty_Lam "X" KB (Ty_Lam "Y" KB (Ty_App (Ty_Var "X") (Ty_Var "Y"))))
+        (Ty_App (Ty_Var "v") (Ty_Var "Y")).
+
+Lemma t3_bad__not_wk :
+    forall Δ Γ,
+        (Δ : Γ ⊢ t3_bad) -> False.
+Proof.
+    intros.
+    unfold t3_bad in H.
+    inversion H; subst; clear H.
+    inversion H2; subst; clear H2.
+    inversion H6; subst; clear H6.
+
+    (*But Y must be in Γ*)
+    inversion H3; subst; clear H3.
+    inversion H2; subst; clear H2.
+
+    contradiction H8 with (X := "Y").
+    all: auto with *.
+    simpl.
+    right.
+    left.
+    reflexivity.
+Qed.
+
+(* This term steps to t3_bad *)
+Definition t4_bad := Ty_App
+    (Ty_Lam "W" KB ( Ty_App
+        (Ty_Lam "X" KB (Ty_Lam "Y" KB (Ty_App (Ty_Var "X") (Ty_Var "Y"))))
+        (Ty_Var "W")
+    ))
+    (Ty_App (Ty_Var "v") (Ty_Var "Y")).
+
+Lemma t4_bad__not_wk :
+    forall Δ Γ,
+        (Δ : Γ ⊢ t4_bad) -> False.
+Proof.
+    intros.
+    unfold t4_bad in H.
+    inversion H; subst; clear H.
+    inversion H2; subst; clear H2.
+    inversion H6; subst; clear H6.
+    inversion H1; subst; clear H1.
+    inversion H11; subst; clear H11.
+
+    (*But Y must be in Γ*)
+    inversion H3; subst; clear H3.
+    inversion H6; subst; clear H6.
+
+    contradiction H13 with (X := "Y").
+    simpl.
+    right. auto.
+    simpl.
+    right. left.
+    reflexivity.
+Qed.
+
+
+(** Kinding of types *)
+Reserved Notation "Δ '|-*' T ':' K" (at level 40, T at level 0, K at level 0).
+Inductive has_kind : list (string * kind) -> ty -> kind -> Prop :=
+  | K_Var : forall Δ X K,
+      lookup X Δ = Some K ->
+      Δ |-* (Ty_Var X) : K
+  | K_Lam : forall Δ X K1 T K2,
+      ((X, K1) :: Δ) |-* T : K2 ->
+      Δ |-* (Ty_Lam X K1 T) : (Kind_Arrow K1 K2)
+  | K_App : forall Δ T1 T2 K1 K2,
+      Δ |-* T1 : (Kind_Arrow K1 K2) ->
+      (drop_btv Δ (btv T1)) |-* T2 : K1 -> (* This rule makes that a well-kinded type can never have capture when evaluated one step*)
+      Δ |-* (Ty_App T1 T2) : K2
+where "Δ '|-*' T ':' K" := (has_kind Δ T K).
+
+Theorem well_kinded__no_capture :
+    (* Maybe:
+        Then if T is well_kinded with above has_kind,
+        then it is also well_kinded with canonical has_kind
+        And that then they normalise to same type?
+
+        Probably, but seems like a lot of work.
+    *) True
+.
+
+
+  (* Usual step relation that has no normality restrictions, 
+    but with naive subsitutions.
+*)
+Inductive step : ty -> ty -> Set :=
+    | step_beta (X : string) (K : kind) (S T : ty) :
+        normal_Ty T ->
+        step (Ty_App (Ty_Lam X K S) T) (substituteT X T S) 
+    | step_appL S1 S2 T :
+        neutral_Ty S1 ->
+        step S1 S2 -> step (Ty_App S1 T) (Ty_App S2 T)
+    | step_appR S T1 T2 :
+        step T1 T2 -> step (Ty_App S T1) (Ty_App S T2)
+    | step_abs bX K T1 T2 :
+        step T1 T2 -> step (Ty_Lam bX K T1) (Ty_Lam bX K T2)
+    .
+
+Fixpoint count (X : string) (T: ty) : nat :=
+    match T with
+    | Ty_Var Y =>
+        if X =? Y then 1 else 0
+    | Ty_Lam Y K T' => 0 (* Not important *)
+    | Ty_App T1 T2 =>
+        count X T1 + count X T2
+    end.
+
+Fixpoint duplicate {A : Type} (l : list A) (n : nat ) := 
+  match n with
+  | O => nil
+  | S n' => (l ++ (duplicate l n'))%list
+  end.
+
+(* collect binders*)
+Fixpoint dsubst' (T : ty) : list (string * ty) :=
+  match T with
+  | Ty_Var X => []
+  | Ty_Lam Y K T_body =>
+    (Y, T_body)::(dsubst' T_body)
+  | Ty_App T1 T2 =>
+    dsubst' T1 ++ dsubst' T2
+  end.
+
+(* This is the property that we want to prove: that the step relation preserves the typing property *)
+
+Fixpoint dsubst (Δ2 : list (string * ty)) (X : string) (U : ty) (T : ty): list (string * ty) :=
+  match T with
+  | Ty_Var Y => if X =? Y then Δ2 else nil
+  | Ty_App T1 T2 => 
+      (dsubst Δ2 X U T1 ++ dsubst Δ2 X U T2)%list
+  | Ty_Lam Y K T_body =>
+    if X =? Y then
+      (Y, T_body)::(dsubst' T_body)
+    else 
+      (Y, substituteT X U T_body)::(dsubst Δ2 X U T_body)
+  end.
+
+Lemma BF_propertyΔ :
+    forall (Δ : list (string * ty)) (Γ : list string) (T : ty) (X : string),
+        Δ : Γ ⊢ T ->
+        In X Γ -> ~ In X (map fst Δ).
+Proof.
+  intros Δ Γ T X Hnd.
+  generalize dependent X.
+  induction Hnd; intros.
+  - auto.
+  - destr_eqb_eq X X0.
+    + unfold P_BF in H.
+      apply H. auto.
+    + simpl. intuition.
+      specialize (IHHnd X0).
+      apply IHHnd.
+      apply in_cons.
+      auto. auto.
+  - rewrite map_app.
+    apply not_in_app. split; eauto.
+Qed.
+
+(* This is the property that we want to prove: that the step relation preserves the typing property *)
+
+(* HMM, I do not seem to use this for open U? *)
+Theorem substituteT_preserves_NoDup : forall T Δ1 Δ2 Γ X U,
+  P_ND2' ((X, T)::Δ1) Δ2 ->
+  P_Dup_Normal ((X, T)::Δ1) Δ2 ->
+  (* P_BF (((X, T)::Δ1) ++ Δ2) Γ -> *)  (* Hopefully we do not need this *)
+  normal_Ty U ->
+  Δ1 : (X :: Γ) ⊢ T ->
+  Δ2 : Γ ⊢ U -> (* This lemma is used where X was in a lambda binder: hence, by the new typing rule, it may not occur free in U*)
+  dsubst Δ2 X U T : Γ ⊢ (substituteT X U T).
+Proof with eauto.
+    
+    intros T Δ1 Δ2 Γ X U HPND2 HDupNo HNo HndT HndU.
+    generalize dependent Δ2.
+    generalize dependent Δ1.
+    generalize dependent Γ.
+    generalize dependent U.
+    
+    induction T.
+    - (* Var *)
+      intros.
+      simpl.
+      destr_eqb_eq X s.
+      + inversion HndT; subst.
+        unfold dsubst. auto.
+      + inversion HndT; subst.
+        constructor.
+        inversion HndT.
+        subst.
+        inversion H3; subst.
+        congruence.
+        auto.
+    - (* Lam *)
+      intros.
+      
+      simpl.
+      destr_eqb_eq X s.
+      + (* X = s*)
+        exfalso.
+        inversion HndT; subst.
+        unfold P_BF in H5.
+        specialize (H5 s).
+        contradiction H5.
+        apply in_eq. simpl. left. reflexivity.
+      + (* X <> s *)
+        inversion HndT; subst.
+        
+        assert (WK_Dup' Δ (X :: s :: Γ) T).
+        {
+            (* ADMIT: Weakening: cons_permute *)
+            admit.
+        }
+        apply ND_Lam.
+        eapply IHT; eauto.
+        * (* ADMIT:
+        TODO: This is the trickest case.
+          U normal.   U can be of the form .... (λ(s: K). T) ...
+          Then it must have kind >= kind of (λ (s : K). T), since this must be inside of
+          a lambda body. it cannot be in head position by normality.
+        
+             What if X in Δ2? If it appears in there, it must have the exact same form:
+            (X, Ty_Lam s k T), but that cannot be well-kinded... the argument must have smaller kind
+
+            We cannot hide it in a const function or something: it is normal.
+          *)
+          admit.
+        * (* ADMIT: By above, X cannot occur in Δ2, hence this hold trivially by above*)
+           admit.
+        * (* ADMIT: Weakening Gamma *) admit.
+        * (* hmm, new case.
+        
+            
+          *)
+          unfold P_BF.
+          intros.
+          simpl.
+          intuition.
+          -- subst.
+             unfold P_BF in H6.
+             specialize (H6 X0).
+             contradiction H6.
+             apply in_cons. auto. simpl. left. reflexivity.
+          -- (* By P_BF we know X0 not in the binders of T (i.e. Δ)
+              What about Δ2?
+              Can only happen if X free in T.
+              
+              So we would need: P_BF Δ2 Γ
+            *)
+            apply BF_propertyΔ with (X := X0) in HndU.
+            (* Then we know X0 notin map fst Δ2!*)
+            admit.
+            auto.
+    - intros.
+      simpl.
+      inversion HndT; subst.
+      assert (dsubst Δ2 X U (Ty_App T1 T2) = (dsubst Δ2 X U T1 ++ dsubst Δ2 X U T2)%list).
+      {
+        simpl. reflexivity.
+      }
+      constructor; eauto.
+      + eapply IHT1; eauto.
+        * (* ADMIT:
+            By P_ND2', if X in Δ2, then it is in there with (X, Ty_App T1 T2).
+               That cannot be, that must be ill-kinded, since it is normal?
+
+            Tricky tricky tricky (see also lam case):
+            App case. Kind of U is smaller than kind of T1. So then how can the whole of 
+              Ty_App T1 T2 be in U? It must then be normal (T1 neutral). Hence in whatever
+              term, by normality, its kind will occur in the final kind: it cannot be 
+              removed with some smart function or something, this is vague.
+
+          *)
+           admit.
+        * (* See above, X cannot be in there.*)
+          admit.
+      + eapply IHT2; eauto.
+        * (* ADMIT: see above *) admit.
+        * (* ADMIT: see above *) admit.
+      + (* Everything in Δ2 must for sure be normal, it will be in both sides.
+            I think that it is by normality of U.
+          Suppose (X, T) is a type in Δ0.
+
+          If also (X, T') in Δ3, then T = T'.
+          Then we substitute in identical terms, should be no problem.
+
+          If X not in Δ3, but X in Δ2? By:
+            P_Dup_Normal Δ0 Δ2
+            and P_Dup_Normal Δ3 Δ2
+          *)
+      
+      
+        (* Unsure*) admit.
+      + (* See above *)
+
+        (* Unsure *) admit.
+      + (*
+          P_BF will decompose over app.
+          Then dsubst will never have more binders than Δ0, Δ2, Δ3, U, added,
+          and they all have no binders that are free in Γ by assumption.
+            (Suppose U has a binder, then that binder is also in Δ2.)
+        *)
+      
+        (* Unsure *) admit.
+
+Admitted.
+
+(* This is the property that we want to prove: that the step relation preserves the typing property *)
+Theorem preservation' T1 T2 Δ Γ :
+    Δ : Γ ⊢ T1 -> step T1 T2 -> exists Δ', Δ' : Γ ⊢ T2.
+Proof.
+    intros Hnd Hstep.
+    generalize dependent Δ.
+    generalize dependent Γ.
+    induction Hstep; intros.
+    - inversion Hnd; subst; clear Hnd.
+      inversion H1; subst; clear H1.
+
+      (* What do we know:
+        T is WF under Δ2.
+        T normal.
+        Δ : (X :: Γ) ⊢ S,  so X free in S.
+        We know, if X in Δ2, then S is normal.
+        So why would this hold?
+        Ftvs are not changed by substituteT, so let's ignore Gamma?
+
+        From
+          Δ : (X :: Γ) ⊢ S
+
+          we should conclude
+
+          f(Δ) : Γ ⊢ substituteT X T S
+
+        I think maybe we know that (X, S)::Δ contains no duplicates.
+          I think that follows from Δ : (X :: Γ) ⊢ S, the BF property.
+        
+        Let's say S = λY. (λZ. Y X) (λV. X)
+        Then Δ = (Y, (λZ. Y X) (λV. X)) :: (Z, Y X) :: (V, X) :: nil)).
+        
+        This term would become (substituteT X T S) = (λY. (λZ. Y T) (λV. T)),
+        but T the binders of T (say T = λW. W) should be carefully included into Δ.
+
+        If T = λW. W, then substituteT X T S =
+          (λY. (λZ. Y (λW. W)) (λV. (λW. W)))
+        Which must have
+          (Y, (λZ. Y (λW. W)) (λV. (λW. W))) :: (Z, Y (λ W. W))
+            :: (W, W)
+            :: (V, (λ W. W))
+            :: (W, W)
+           :: nil)).
+          
+        Maybe we can find some algorithm for that?
+        We traverse Δ, whenever we see X, replace with T.
+        Whenever in this entry X is not surrounded by a lambda anymore,
+        add new entries Δ2
+
+        So it is a function f(Δ, Δ2, X, T) that returns Δ'.
+
+        But why would we have the properties?
+
+
+      *)
+      assert (dsubst Δ2 X T S : Γ ⊢ (substituteT X T S)).
+      {
+        eapply substituteT_preserves_NoDup; eauto.
+      }
+      exists (dsubst Δ2 X T S)%list.
+      assumption.
+      
+    - (* Analogous to below *)
+      admit.
+    - inversion Hnd; subst.
+      specialize (IHHstep Γ Δ2 H2) as [Δ2' Hnd2'].
+      exists (Δ1 ++ Δ2')%list.
+      constructor; auto.
+      + (* Something, say (X, T) in Δ2' stepped. so we could have lost this property if 
+            X is a key in Δ1. 
+            But by P_Dup_Normal, we know that then it could not have stepped (by normality).
+        *)
+        admit.
+      + (* P_DUP ? *)
+        admit.
+      + (* Δ2' is obtained from Δ2 by stepping. Hence bvs Δ2' are subset of bvs Δ2, so no problem*)
+        admit.
+    - inversion Hnd; subst.
+      specialize (IHHstep (bX :: Γ) Δ0 H2) as [Δ0' Hnd0'].
+      exists ((bX, T2)::Δ0')%list.
+      constructor; auto.
+Admitted.
+
+(* Even after stepping, the type is still typeable in the more restrictive TyApp rule
+  meaning that even after stepping, when stepping again, we will again not have capture
+  i.e. this is the property that GU implies that is preserved
+  under normalisation/betaReduction.
+*)
+Theorem preservation T1 T2 Δ K :
+    Δ |-* T1 : K -> step T1 T2 -> Δ |-* T2 : K.
+Proof.
+    intros Hwk Hstep.
+    generalize dependent Δ.
+    generalize dependent K.
+    induction Hstep; intros.
+    - inversion Hwk; subst.
+      inversion H2; subst.
+      assert ((drop_btv Δ (btv S)) |-* T : K1).
+      {
+        (* Weakening, we coulud potentially add X, but it cannot be free in T by H4*)
+        admit.
+      }
+      eapply substituteT_preserves_kinding; eauto.
+    - inversion Hwk; subst.
+      apply K_App with (K1 := K1).
+      + eapply IHHstep; eauto.
+      + (* stepping does not introduce new btvs, 
+        but it could remove them, hence
+            btv S2  subset of  btv S1
+
+            Hence 
+               inclusion (drop_btv Δ (btv s1)) (drop_btv Δ (btv s2))
+            reasoning: btv s1 is bigger than btv s2: we remove more, hence lookup in the first implies still lookup in the second, which has every element in the first, and possibly more
+
+            But what about shadowing??? I fear the existence of an X that becomes visible, but then that X was not necessary to begin with. So no issue.
+
+        *)
+        admit.
+    - inversion Hwk; subst.
+      apply K_App with (K1 := K1).
+      + assumption.
+      + eapply IHHstep; eauto.
+    - inversion Hwk; subst.
+      constructor.
+      eapply IHHstep; eauto.
+      
+Admitted.
