src/PlutusIR/Semantics/Static/typing_nc_prototype.v
@@ -1,0 +1,857 @@
+From Coq Require Import Lists.List.
+From Coq Require Import Strings.String.
+
+From PlutusCert Require Import Util.List util.
+
+Import ListNotations.
+Local Open Scope list_scope.
+Local Open Scope string_scope.
+
+
+(** kinds *)
+Inductive kind :=
+  | Kind_Base : kind
+  | Kind_Arrow : kind -> kind -> kind.
+
+(** Types *)
+Inductive ty :=
+  | Ty_Var : string -> ty
+  | Ty_Lam : string -> kind -> ty -> ty
+  | Ty_App : ty -> ty -> ty
+  | Ty_Forall : string -> kind -> ty -> ty
+  | Ty_Fun : ty -> ty -> ty
+.
+
+Fixpoint btv (T : ty) : (list string) :=
+    match T with
+    | Ty_Var x => []
+    | Ty_Lam x K T0 => x :: (btv T0)
+    | Ty_App T1 T2 => btv T1 ++ btv T2
+    | Ty_Forall x K T0 => x :: (btv T0)
+    | Ty_Fun T1 T2 => btv T1 ++ btv T2
+    end.
+
+
+  Function ftv (T : ty) : list string :=
+    match T with
+    | Ty_Var X =>
+        [X]
+    | Ty_Fun T1 T2 =>
+        ftv T1 ++ ftv T2
+    | Ty_Forall X K T' =>
+        remove string_dec X (ftv T')
+    | Ty_Lam X K1 T' =>
+        remove string_dec X (ftv T')
+    | Ty_App T1 T2 =>
+        ftv T1 ++ ftv T2
+    end.
+
+Module Ty.
+  Definition closed (T : ty) :=
+    forall X, ~ In X (ftv T).
+End Ty.
+
+Fixpoint drop_btv (Δ : list (string * kind)) (btvs : list string) : list (string * kind) :=
+    match Δ with
+    | ((X, K)::Δ') => 
+                    if (in_dec string_dec X btvs) then
+                        (drop_btv Δ' btvs)
+                      else
+                        ((X, K)::(drop_btv Δ' btvs))
+    | nil => nil
+    end.
+
+(** Kinding of types *)
+Reserved Notation "Δ '|-*' T ':' K" (at level 40, T at level 0, K at level 0).
+Inductive has_kind : list (string * kind) -> ty -> kind -> Prop :=
+  | K_Var : forall Δ X K,
+      lookup X Δ = Some K ->
+      Δ |-* (Ty_Var X) : K
+  | K_Lam : forall Δ X K1 T K2,
+      ((X, K1) :: Δ) |-* T : K2 ->
+      Δ |-* (Ty_Lam X K1 T) : (Kind_Arrow K1 K2)
+  | K_App : forall Δ T1 T2 K1 K2,
+      Δ |-* T1 : (Kind_Arrow K1 K2) ->
+      Δ |-* T2 : K1 -> (* This rule makes that a well-kinded type can never have capture when evaluated one step*)
+      Δ |-* (Ty_App T1 T2) : K2
+  | K_Forall : forall Δ X K T,
+      ((X, K) :: Δ) |-* T : Kind_Base ->
+      Δ |-* (Ty_Forall X K T) : Kind_Base
+  | K_Fun : forall Δ T1 T2,
+      Δ |-* T1 : Kind_Base ->
+      Δ |-* T2 : Kind_Base ->
+      Δ |-* (Ty_Fun T1 T2) : Kind_Base
+where "Δ '|-*' T ':' K" := (has_kind Δ T K).
+
+Theorem well_kinded__no_capture :
+    (* Maybe:
+        Then if T is well_kinded with above has_kind,
+        then it is also well_kinded with canonical has_kind
+        And that then they normalise to same type?
+
+        Probably, but seems like a lot of work.
+    *) True
+.
+
+(* Maybe instead: if T is well_kinded and an application, then there is no capture*)
+(* Theorem well_kinded__no_capture2 Δ T1 T2 K :
+    (Δ |-* (Ty_App T1 T2) : K) -> (In X (ftv T2)) -> (~ In X (btv T1)). *)
+
+Fixpoint substituteT (X : string) (U T : ty) : ty :=
+  match T with
+  | Ty_Var Y =>
+    if X =? Y then U else Ty_Var Y
+  | Ty_Lam Y K1 T' =>
+    if X =? Y then Ty_Lam Y K1 T' else Ty_Lam Y K1 (substituteT X U T')
+  | Ty_App T1 T2 =>
+    Ty_App (substituteT X U T1) (substituteT X U T2)
+  | Ty_Forall Y K T' =>
+    if X =? Y then Ty_Forall Y K T' else Ty_Forall Y K (substituteT X U T')
+    | Ty_Fun T1 T2 =>
+    Ty_Fun (substituteT X U T1) (substituteT X U T2)
+  end.
+
+(* HMM, I do not seem to use this for open U? *)
+Theorem substituteT_preserves_kinding : forall T Delta X K U L,
+  ((X, L) :: Delta) |-* T : K ->
+  nil |-* U : L -> 
+  Delta |-* (substituteT X U T) : K.
+Proof with eauto.
+  induction T.
+  all: intros Delta X K U L Hkind__T HHkind__U.
+  all: simpl.
+  all: inversion Hkind__T; subst...
+  - (* Ty_Var *)
+    destruct (X =? s)%string eqn:Heqb.
+    + (* X = Y *)
+      apply eqb_eq in Heqb as Heq.
+      subst.
+      assert (K = L).
+      {
+        simpl in H1.
+        rewrite Heqb in H1.
+        inversion H1; auto.
+      }
+      subst.
+      (* ADMIT: weakening empty *)
+      admit.
+    + (* X <> Y *)
+      apply eqb_neq in Heqb as Hneq.
+      rewrite lookup_neq in H1...
+      constructor.
+      assumption.
+  - (* Ty_Lam *)
+    rename s into bX.
+    destruct (X =? bX)%string eqn:Heqb.
+    + (* X = bX *)
+      apply eqb_eq in Heqb as Heq.
+      subst.
+      apply K_Lam...
+      (* ADMIT: Weakening shadow *)
+      admit.
+    + (* X <> bX *)
+      apply eqb_neq in Heqb as Hneq.
+      apply K_Lam.
+      eapply IHT...
+      (* ADMIT: Weakening cons permute *)
+      admit.
+  - (* Ty_App *)
+    econstructor; eauto.
+  - (* Ty_Forall *)
+    rename s into bX.
+    destruct (X =? bX)%string eqn:Heqb.
+    + (* X = bX *)
+      apply eqb_eq in Heqb as Heq.
+      subst.
+      apply K_Forall...
+      (* ADMIT: Weakening shadow *)
+      admit.
+    + (* X <> bX *)
+      apply eqb_neq in Heqb as Hneq.
+      apply K_Forall.
+      eapply IHT...
+      (* ADMIT: Weakening cons permute *)
+      admit.
+  - (* Ty_Fun *)
+    econstructor; eauto.
+Admitted.
+
+
+(* Usual step relation that has no normality restrictions, 
+    but with naive subsitutions.
+*)
+Inductive step : ty -> ty -> Set :=
+    | step_beta (X : string) (K : kind) (S T : ty) :
+        step (Ty_App (Ty_Lam X K S) T) (substituteT X T S) 
+    | step_appL S1 S2 T :
+        step S1 S2 -> step (Ty_App S1 T) (Ty_App S2 T)
+    | step_appR S T1 T2 :
+        step T1 T2 -> step (Ty_App S T1) (Ty_App S T2)
+    | step_abs bX K T1 T2 :
+        step T1 T2 -> step (Ty_Lam bX K T1) (Ty_Lam bX K T2)
+    | step_funL S1 S2 T :
+        step S1 S2 -> step (Ty_Fun S1 T) (Ty_Fun S2 T)
+    | step_funR S T1 T2 :
+        step T1 T2 -> step (Ty_Fun S T1) (Ty_Fun S T2)
+    | step_forall K bX T1 T2 :
+        step T1 T2 -> step (Ty_Forall bX K T1) (Ty_Forall bX K T2)
+    .
+
+(* Even after stepping, the type is still typeable in the more restrictive TyApp rule
+  meaning that even after stepping, when stepping again, we will again not have capture
+  i.e. this is the property that GU implies that is preserved
+  under normalisation/betaReduction.
+*)
+Theorem preservation T1 T2 Δ K :
+    Δ |-* T1 : K -> step T1 T2 -> Δ |-* T2 : K.
+Proof.
+    intros Hwk Hstep.
+    generalize dependent Δ.
+    generalize dependent K.
+    induction Hstep; intros.
+    - inversion Hwk; subst.
+      inversion H2; subst.
+      (* By weakening we have Δ |-* T : K1 then by substituteT_preserves_kinding (should also hold for open U, see substituteTCA_preserves_kinding) *)
+      admit.
+    - inversion Hwk; subst.
+      apply K_App with (K1 := K1).
+      + eapply IHHstep; eauto.
+      + (* stepping does not introduce new btvs, 
+        but it could remove them, hence
+            btv S2  subset of  btv S1
+
+            Hence 
+               inclusion (drop_btv Δ (btv s1)) (drop_btv Δ (btv s2))
+            reasoning: btv s1 is bigger than btv s2: we remove more, hence lookup in the first implies still lookup in the second, which has every element in the first, and possibly more
+
+            But what about shadowing??? I fear the existence of an X that becomes visible, but then that X was not necessary to begin with. So no issue.
+
+        *)
+        admit.
+    - inversion Hwk; subst.
+      apply K_App with (K1 := K1).
+      + assumption.
+      + eapply IHHstep; eauto.
+    - inversion Hwk; subst.
+      constructor.
+      eapply IHHstep; eauto.
+    - (* Analogous to appL *)
+      admit.
+    - (* Analogous to appR *)
+      admit.
+    - (* Analogous to abs *)
+      admit.     
+Admitted.
+
+(* Mock normaliser without beta reduction*)
+Fixpoint normaliser (T : ty) : option ty :=
+  match T with
+  | Ty_Var _ => Some T
+  | Ty_Lam x K T' =>
+    match normaliser T' with
+    | Some Tn => Some (Ty_Lam x K Tn)
+    | None => None
+    end
+  | Ty_App T1 T2 =>
+    match normaliser T1, normaliser T2 with
+    | Some T1n, Some T2n => Some (Ty_App T1n T2n)
+    | _, _ => None
+    end
+  | Ty_Forall x K T' =>
+    match normaliser T' with
+    | Some Tn => Some (Ty_Forall x K Tn)
+    | None => None
+    end
+  | Ty_Fun T1 T2 =>
+    match normaliser T1, normaliser T2 with
+    | Some T1n, Some T2n => Some (Ty_Fun T1n T2n)
+    | _, _ => None
+    end
+  end.
+
+
+(*******   Terms and their types   ******)
+Inductive term :=
+  | Var      : string -> term
+  | TyAbs    : string -> kind -> term -> term
+  | LamAbs   : string -> ty -> term -> term
+  | Apply    : term -> term -> term
+  | TyInst   : term -> ty -> term.
+
+
+Fixpoint drop_ty_var' X (Γ : list (string * ty)) (acc : list string): list (string * ty) :=
+  match Γ with
+  | nil => nil
+  | (x, T) :: Γ' =>
+      if (in_dec string_dec X (ftv T)) then 
+        drop_ty_var' X Γ' (x::acc)
+      else if in_dec string_dec x acc then
+        drop_ty_var' X Γ' acc
+      else (x, T) :: drop_ty_var' X Γ' acc
+  end.
+
+Definition drop_ty_var X (Γ : list (string * ty)) : list (string * ty) :=
+  drop_ty_var' X Γ nil.
+
+
+Reserved Notation "Delta ',,' Gamma '|-+' t ':' T" (at level 101, t at level 0, T at level 0, no associativity).
+Inductive has_type : list (string * kind) -> list (string * ty) -> term -> ty -> Prop :=
+  (* Simply typed lambda caclulus *)
+  | T_Var : forall Γ Δ x T Tn,
+      lookup x Γ = Coq.Init.Datatypes.Some T ->
+      Δ |-* T : Kind_Base ->
+      normaliser T = Some Tn ->
+      Δ ,, Γ |-+ (Var x) : Tn
+  | T_LamAbs : forall Δ Γ x T1 t T2n T1n,
+      Δ |-* T1 : Kind_Base ->
+      normaliser T1 = Some T1n ->
+      Δ ,, (x, T1n) :: Γ |-+ t : T2n ->
+      Δ ,, Γ |-+ (LamAbs x T1 t) : (Ty_Fun T1n T2n)
+  | T_Apply : forall Δ Γ t1 t2 T1n T2n,
+      Δ ,, Γ |-+ t1 : (Ty_Fun T1n T2n) ->
+      Δ ,, Γ |-+ t2 : T1n ->
+      Δ ,, Γ |-+ (Apply t1 t2) : T2n
+  (* Universal types *)
+  | T_TyAbs : forall Δ Γ X K t Tn,
+      ((X, K) :: Δ) ,, (drop_ty_var X Γ) |-+ t : Tn ->
+      Δ ,, Γ |-+ (TyAbs X K t) : (Ty_Forall X K Tn)
+  | T_TyInst : forall Δ Γ t1 T2 T1n X K2 T0n T2n,
+      Δ ,, Γ |-+ t1 : (Ty_Forall X K2 T1n) ->
+      (drop_btv Δ (btv T1n)) |-* T2 : K2 ->
+      normaliser T2 = Some T2n ->
+      normaliser (substituteT X T2n T1n) = Some T0n ->
+      Δ ,, Γ |-+ (TyInst t1 T2) : T0n
+where "Δ ',,' Γ '|-+' t ':' T" := (has_type Δ Γ t T).
+
+
+Fixpoint subst (x : string) (s : term) (t : term) : term :=
+  match t with
+  | Var y =>
+      if x =? y
+        then s
+        else Var y
+  | TyAbs bX K t0 =>
+      TyAbs bX K (subst x s t0)
+  | LamAbs bx T t0 =>
+      if x =? bx
+        then LamAbs bx T t0
+        else LamAbs bx T (subst x s t0)
+  | Apply t1 t2 =>
+      Apply (subst x s t1) (subst x s t2)
+  | TyInst t0 T =>
+      TyInst (subst x s t0) T
+  end.
+Notation "'[' x ':=' s ']' t" := (subst x s t) (at level 20, x constr).
+
+
+Fixpoint substA (X : string) (U : ty) (t : term) {struct t} : term :=
+  match t with
+  | Var y =>
+      Var y
+  | TyAbs bX K t0 =>
+      if X =? bX
+        then TyAbs bX K t0
+        else TyAbs bX K (substA X U t0)
+  | LamAbs bx T t0 =>
+      LamAbs bx (substituteT X U T) (substA X U t0)
+  | Apply t1 t2 =>
+      Apply (substA X U t1) (substA X U t2)
+  | TyInst t0 T =>
+      TyInst (substA X U t0) (substituteT X U T)
+  end.
+Notation "':[' X ':=' U ']' t" := (substA X U t) (at level 20, X constr).
+
+
+Reserved Notation "t '=[' j ']=>' v"(at level 40).
+Inductive eval : term -> term -> nat -> Prop :=
+  | E_LamAbs : forall j x T t,
+      j = 0 ->
+      LamAbs x T t =[j]=> LamAbs x T t
+  | E_Apply : forall j t1 t2 x T t0 v2 v0 j1 j2 j0,
+      j = j1 + j2 + 1 + j0 ->
+      t1 =[j1]=> LamAbs x T t0 ->
+      t2 =[j2]=> v2 ->
+      ([x := v2 ] t0 ) =[j0]=> v0 ->
+      Apply t1 t2 =[j]=> v0
+  (** Universal types *)
+  | E_TyAbs : forall j X K t,
+      j = 0 ->
+      TyAbs X K t =[j]=> TyAbs X K t
+  | E_TyInst : forall j t1 T2 X K t0 v0 j1 j0,
+      j = j1 + 1 + j0 ->
+      t1 =[j1]=> TyAbs X K t0 ->
+      (:[X := T2] t0) =[j0]=> v0 ->
+      TyInst t1 T2 =[j]=> v0
+where "t '=[' j ']=>' v" := (eval t v j).
+
+
+(* TERM SUBSTITUTION PRESERVATION *)
+
+Lemma substitution_preserves_typing :
+  forall Delta Gamma x U Un v T t,
+    Delta ,, ((x, U) :: Gamma) |-+ t : T ->
+    normaliser U = Some Un ->
+    nil ,, nil |-+ v : Un ->
+    Delta ,, Gamma |-+ ([x := v] t) : T.
+Proof with eauto.
+    intros.
+    generalize dependent Delta.
+    generalize dependent Gamma.
+    generalize dependent T.
+    induction t; intros.
+  all: intros; autounfold; intros.
+  all: try solve [try (inversion H || inversion H0 || inversion H1); subst; eauto with typing].
+  - (* Var *)
+    simpl.
+    destruct (x =? s)%string eqn:Heqb.
+    + apply eqb_eq in Heqb as Heq.
+      subst.
+      inversion H; subst.
+      simpl in H3.
+      rewrite Heqb in H3.
+      inversion H3; subst; clear H3.
+      assert (Un = T).
+      { (*ADMIT: normalisation__deterministic *)admit. }
+      subst.
+      (* ADMIT: Weakening empty *)
+      admit.
+    + apply eqb_neq in Heqb as Hneq.
+      inversion H. subst.
+      eapply T_Var...
+      simpl in H3.
+      rewrite Heqb in H3...
+  - (* TyAbs *)
+    simpl.
+    inversion H; subst.
+    apply T_TyAbs; auto.
+    eapply IHt...
+    destr_eqb_eq s x.
+    + (* ADMIT:
+        (* t typeable without x, so also with x by weakening*)
+      *)
+      admit.
+    + (* ADMIT: drop_ty_var s ((x, U)...) unfolds to goal*)
+      admit.
+  - (* LamAbs *)
+    inversion H. subst.
+    simpl.
+    destruct (x =? s)%string eqn:Heqb.
+    + apply eqb_eq in Heqb as Heq.
+      subst.
+      apply T_LamAbs...
+      (* ADMIT:  By H10: Delta,, (s, T1n) :: (s, U) :: Gamma |-+ t0 : T2n 
+             and weakening *)
+      admit.
+    + apply eqb_neq in Heqb as Hneq.
+      apply T_LamAbs...
+      eapply IHt...
+      (* ADMIT: By H10 and weakening swap/ cons permute *)
+      admit.
+  - (* Apply *)
+    simpl.
+    inversion H; subst.
+    eapply T_Apply...
+  - (* TyInst *)
+     simpl.
+     inversion H; subst.
+     eapply T_TyInst...
+(* ADMIT: See admits above*)
+Admitted.
+
+Definition gsubst (a : string) (T' : ty ) (Gamma : list (string * ty)) :=
+  map (fun '(x, T) => (x, substituteT a T' T)) Gamma.
+
+Lemma gsubst_empty : forall X U,
+    gsubst X U nil = nil.
+Proof.
+  intros X U.
+  unfold gsubst.
+  simpl.
+  reflexivity.
+Qed.
+
+Lemma gsubst__substituteT Gamma x X U T :
+    lookup x Gamma = Datatypes.Some T ->
+    lookup x (gsubst X U Gamma) = Datatypes.Some (substituteT X U T).
+Proof with auto.
+  induction Gamma.
+  all: intros H; unfold gsubst.
+  - inversion H.
+  - destruct a.
+    destruct (string_dec x s).
+    + subst s.
+      simpl.
+      rewrite eqb_refl.
+      rewrite lookup_eq in H.
+      congruence.
+    + rewrite lookup_neq in H...
+      apply eqb_neq in n.
+      rewrite eqb_sym in n.
+      simpl.
+      rewrite n...
+Qed.
+
+Lemma gsubst_absorbs_substituteT : forall x X U T Gamma,
+    ((x, (substituteT X U T)) :: gsubst X U Gamma) = gsubst X U ((x, T) :: Gamma).
+Proof.
+  reflexivity.
+Qed.
+
+
+Lemma drop_ty_var__gsubst s X U Γ : 
+  s <> X ->
+  Ty.closed U ->
+  drop_ty_var s (gsubst X U Γ) = gsubst X U (drop_ty_var s Γ).
+Proof.
+  intros Hneq Hclosed.
+  unfold drop_ty_var.
+  remember (nil) as R.
+  clear HeqR.
+  generalize dependent R.
+  induction Γ; intros.
+  - simpl.
+    reflexivity.
+  - destruct a as [x T].
+    simpl.
+    destruct (in_dec string_dec s
+      (ftv
+      (substituteT X U T))).
+    + destruct (in_dec string_dec s (ftv T)).
+      * eapply IHΓ.
+      * exfalso.
+        (* ADMIT: s in substT X U T, but U is closed, so s in T. *)
+        admit.
+    + 
+      destruct (in_dec string_dec s (ftv T)).
+      * exfalso.
+        (* ADMIT: s not in substT X U T 
+                  by s <> X, then s not in T *)
+        admit.
+      * destruct (in_dec string_dec x R).
+        -- eapply IHΓ.
+        -- rewrite <- gsubst_absorbs_substituteT.
+           f_equal.
+           eapply IHΓ.
+(* ADMIT: See comments *)    
+Admitted.
+
+Lemma substituteT__normalisation T Tn SubTn X U:
+  normaliser T = Some Tn ->
+  normaliser (substituteT X U Tn) = Some SubTn ->
+  normaliser (substituteT X U T) = Some SubTn.
+Proof.
+  (* I think this could be problematic if U has ftvs
+    Let U = TyVar Z.
+
+    We are substituting X.
+
+    Let T = TyApp (TyLam X K (TyLam V K (TyVar V)) (X * V).
+    Then Tn = TyLam V' K V'.
+
+    substituteT X U T = TyApp (TyLam X K (TyLam V K (TyVar V)) (Z * V).
+      normalises to
+        TyLam V'' K (TyVar V'')
+        where V'' is different fresh than V', because it is based on ftvs in U = Z <> X
+    
+    substitueT X U Tn = TyLam V' K V'
+
+
+  *)
+Admitted.
+
+(* We need this lemma for open U by substA. Does it hold?*)
+Lemma substituteT__normalisation2 T SubTn X U Un :
+  normaliser U = Some Un ->
+  normaliser (substituteT X U T) = Some SubTn ->
+  normaliser (substituteT X Un T) = Some SubTn.
+Proof.
+  (*
+    Suppose U = λ (P:K).   ((λ (Y:K). λ (V:K). V) * (P * V))
+    Then Un = λ (P: K).     λ (V':K). (P * V)
+
+    T = X * G
+
+    substituteT X U T =   λ (P:K).   ((λ (Y:K). λ (V:K). V) * (P * V))   *  G
+        ---> ((λ (Y:K). λ (V:K). V) * (G * V))
+        ---> λ (V'':K). (G * V'')  
+
+    substituteT X Un T = λ (P: K).     λ (V':K). (P * V)    *  G
+        ---> λ (V':K). (G * V')
+
+      (* Different V' and V''  !!!*)
+  *)
+Admitted.
+
+
+(* We also know U is closed, but do not need it yet *)
+Lemma commute_substituteT :
+  forall X U V T,
+    substituteT X U (substituteT X V T) = substituteT X (substituteT X U V) T.
+Proof.
+  intros X U V T.
+  induction T.
+  - simpl.
+    destr_eqb_eq X s; auto.
+    simpl.
+    apply eqb_neq in H; rewrite H; auto.
+  - simpl.
+    destr_eqb_eq X s; auto.
+    simpl.
+    rewrite String.eqb_refl; auto.
+    simpl.
+    apply eqb_neq in H; rewrite H; auto.
+    f_equal.
+    apply IHT; auto.
+  - simpl.
+    f_equal.
+    apply IHT1; auto.
+    apply IHT2; auto.
+  - simpl.
+    destr_eqb_eq X s; auto.
+    simpl.
+    rewrite String.eqb_refl; auto.
+    simpl.
+    apply eqb_neq in H; rewrite H; auto.
+    f_equal.
+    apply IHT; auto.
+  - simpl.
+    f_equal.
+    apply IHT1; auto.
+    apply IHT2; auto.
+Qed.
+
+Theorem substA_preserves_typing :
+    forall Delta Gamma X K U T Tn t,
+    ((X, K) :: Delta) ,, Gamma |-+ t : T ->
+    nil |-* U : K ->
+    normaliser (substituteT X U T) = Some Tn ->
+    Delta ,, (gsubst X U Gamma) |-+ ( :[X := U] t ): Tn.
+Proof with (eauto using substituteT_preserves_kinding with typing).
+  intros.
+  generalize dependent Delta.
+  generalize dependent Gamma.
+  generalize dependent T.
+  generalize dependent Tn.
+  induction t.
+  all: try (intros Tn T Hnorm__Tn Gamma Delta Htyp__t).
+  all: try (inversion Htyp__t; subst).
+  - (* Var *)
+    simpl.
+    (*
+      lookup s Gamma = Some T0   (* T_Var*)
+      normalise T0 T             (* T_Var *)
+
+      normalise (substituteT X U T) Tn  (* P_Term *)
+    *)
+    apply T_Var with (T := (substituteT X U T0)).
+    + eapply gsubst__substituteT; eauto.
+    + eapply substituteT_preserves_kinding; eauto.
+    + eapply substituteT__normalisation; eauto.
+  - (* TyAbs *)
+    simpl.
+    destr_eqb_eq X s.
+    + (* X = s *)
+      simpl substituteT in Hnorm__Tn.
+      rewrite eqb_refl in Hnorm__Tn.
+      inversion Hnorm__Tn; subst.
+      destruct_match.
+      inversion H1; subst; clear H1.
+      constructor.
+      assert (Tn0 = t0).
+      {
+        (* ADMIT: has_type__normal*)
+        admit.
+      }
+      subst.
+      (* ADMIT: 
+        t typeable without s,
+        so the keys in Gamma that have values with s, are not
+        free in t.
+        so if we substitute s with U, then this does nothing
+        still we can remove it then with drop_ty_var.
+        see also annotationSubstitution.v
+      *)
+      admit.
+    + simpl substituteT in Hnorm__Tn.
+      apply eqb_neq in H.
+      assert (X <> s) by now apply eqb_neq in H.
+      rewrite H in Hnorm__Tn.
+      inversion Hnorm__Tn; subst.
+      destruct_match.
+      inversion H3; subst; clear H3.
+      constructor.
+      rewrite drop_ty_var__gsubst; auto.
+      * eapply IHt; eauto.
+        (* ADMIT: Weakening swap *)
+        admit.
+      * (* ADMIT: U closed*)
+        admit.
+  - (* LamAbs *)
+    simpl.
+    simpl substituteT in Hnorm__Tn.
+    inversion Hnorm__Tn; subst.
+    repeat destruct_match.
+    inversion H1; subst; clear H1.
+    constructor; auto.
+    * eapply substituteT_preserves_kinding; eauto.
+    * eapply substituteT__normalisation; eauto.
+    * assert ((s, substituteT X U T1n) :: gsubst X U Gamma = gsubst X U ((s, T1n) :: Gamma)).
+      {
+        rewrite gsubst_absorbs_substituteT; auto.
+      }
+      assert ( Hgsubst_not_normal :
+        (s, (substituteT X U T1n)) :: (gsubst X U Gamma) = 
+          (s, t1) :: gsubst X U Gamma).
+      {
+      (* ADMIT: substituteT X U T1n may not be normal, 
+          how to reconcile? Must gsubst also normalise? 
+          Maybe find counterexample tomorrow.
+
+          Or does typing context not have to be normal?
+          Something like, if it is well_typed for T in gamma,
+          then it is well_typed for Tn in gamma.
+          *)
+          admit.
+      }
+      rewrite <- Hgsubst_not_normal.
+      rewrite H.
+      eapply IHt; eauto.
+  - (* Apply *)
+    simpl.
+    assert (Delta |-* (substituteT X U T1n) : Kind_Base).
+    {
+      eapply substituteT_preserves_kinding; eauto.
+      (* ADMIT: has_type base_kinded*)
+      admit.
+    }
+      
+    econstructor.
+    2: {
+      apply IHt2 with (T := T1n).
+      (*ADMIT:  By strong normalization, this must exist*)
+      - admit.
+      - eauto.
+    }
+    + 
+      eapply IHt1; eauto.
+      simpl substituteT.
+      (* ADMIT: By strong normalization, there is a type that
+        substituteT X U T1n normalises to *)
+      admit.
+  - (* TyInst *)
+    simpl.
+    destr_eqb_eq X X0.
+    + (* X = X0 *)
+      assert (exists T1nn, normaliser T1n = Some T1nn) as [T1nn HT1nn].
+      {
+        (* ADMIT: strong normalization and T1n well-kinded*)
+        admit.
+      } 
+      assert (exists subt0, normaliser (substituteT X0 U t0) = Some subt0) as [subt0 Hsubt0].
+        {
+          assert (((Delta) |-* (substituteT X0 U t0) : K2)).
+          {
+            apply substituteT_preserves_kinding with (L := K); auto.
+            - (* ADMIT: Suppose X0 not in btv T1n, then by unfolding,
+              suppose X0 in btv T1n, then by weakening*)
+              admit.
+          }
+          (* ADMIT: strong normalization and substituteT X0 U t0 well-kinded*)
+          admit.
+      }
+
+      econstructor.
+      * eapply IHt; eauto.
+        simpl substituteT.
+        rewrite eqb_refl.
+        simpl.
+        rewrite HT1nn.
+        reflexivity.
+      * eapply substituteT_preserves_kinding; eauto.
+        (* ADMIT: unfold or weakening, but also:
+              btv T1nn subset of btv T1n by normalisation
+              hence also by weakening.
+        *)
+        admit.
+      * eauto.
+      * (* t0 could be open?? Then T2n could be open?? *)
+        rename t0 into T2.
+        assert (T2 = T2n) by admit. clear H6. subst.
+        assert (T1nn = T1n) by admit. clear HT1nn. subst.
+        assert (T = (substituteT X0 T2n T1n)) by admit. clear H8. subst.
+        erewrite commute_substituteT in Hnorm__Tn.
+        (* substituteT X0 U T2n could be open, and T1n can as well, is that a problem?*)
+        apply substituteT__normalisation2 with (U := substituteT X0 U T2n); eauto.
+    + (* X <> X0 *)
+      assert (exists subT1n, normaliser (substituteT X U t0) = Some subT1n) as [subT1n HsubT1n].
+        {
+          (* ADMIT: See above *)
+          admit.
+        }
+
+      assert (exists SubT1nn, normaliser (substituteT X U T1n) = Some SubT1nn) as [SubT1nn HT1nn].
+      {
+        (* ADMIT: See above*)
+        admit.
+      } 
+
+      econstructor.
+      * eapply IHt; eauto.
+        simpl substituteT.
+        apply eqb_neq in H.
+        rewrite H.
+        simpl.
+        rewrite HT1nn.
+        constructor; eauto.
+      * eapply substituteT_preserves_kinding; eauto.
+        (* ADMIT: unfold or weakening, but also:
+            btv SubT1nn subset of btv T1n by 
+              normalisation and U closed!
+            hence also by weakening.
+        *)
+        admit.
+      * eauto.
+      * 
+        (* ADMIT: Something similar to above *)
+        admit.
+Admitted.
+
+
+Theorem eval__type_preservation : forall t T v k,
+    nil ,, nil |-+ t : T ->
+    t =[k]=> v ->
+    (nil ,, nil |-+ v : T).
+Proof.
+    intros t T v k Ht Hbs.
+    generalize dependent T.
+    induction Hbs; intros.
+    - (* E_LamAbs *)
+      exact Ht.
+    - (* E_Apply *)
+      inversion Ht; subst.
+      specialize (IHHbs1 (Ty_Fun T1n T0) H4).
+      inversion IHHbs1; subst.
+      eapply IHHbs3.
+      eapply substitution_preserves_typing; eauto.
+      (* ADMIT: normaliser T = Some T1n, so T1n normal,
+                     then by normalisation__stable
+      *)
+      admit.
+    - (* E_TyAbs *)
+      exact Ht.
+    - (* E_TyInst *)
+      inversion Ht; subst.
+      specialize (IHHbs1 (Ty_Forall X0 K2 T1n) H2).
+      inversion IHHbs1; subst.
+      eapply IHHbs2.
+      assert (nil = gsubst X0 T2 nil).
+      {
+        simpl.
+        reflexivity.
+      }
+      rewrite H.
+      eapply substA_preserves_typing; eauto.
+
+      (* ADMIT: argument T2 normalizes to T2n, and then substituting the whole normalizes to T in assumption *)
+      admit.
+Admitted.
